Test.Minterop.fst
@@ -1,0 +1,45 @@
+module Test.Minterop
+
+open Common
+open IO.Free
+open IO.Effect
+open IIO.Effect
+open MIO.Effect
+open Minterop
+
+val allowed_file : string -> bool
+let allowed_file fnm = match fnm with
+  | "../Makefile" -> false
+  | "Demos.fst" -> true
+  | _ -> false
+
+val allowed_fd : file_descr -> trace -> bool
+let rec allowed_fd fd s0 =
+  match s0 with
+  | [] -> false
+  | EOpenfile fnm (Inl fd') :: t -> if fd = fd' then allowed_file(fnm)
+                                  else allowed_fd fd t
+  | EClose fd' _  :: t -> if fd = fd' then false else allowed_fd fd t
+  | _ :: t -> allowed_fd fd t
+
+let pi : monitorable_prop = (fun s0 action -> 
+  match action with
+  | (| Openfile, fnm |) -> allowed_file(fnm)
+  | (| Read, fd |) -> allowed_fd fd s0
+  | (| Close, fd |) -> allowed_fd fd s0)
+
+// the plugin will be written in GIO (should be ML?)
+let plugin_type = (pi:monitorable_prop) -> file_descr -> IIO unit pi (fun _ -> True) (fun _ _ _ -> True)
+
+// import plugin_type 
+let webserver (plugin:plugin_type) : IIO unit pi (fun _ -> True) (fun _ _ _ -> True) =
+  rev_append_rev_append ();
+  let fd = static_cmd pi Openfile "Demos.fst" in
+  plugin pi fd
+
+let plugin1 : file_descr -> MIO unit = fun fd ->
+  unsafe_cmd Close fd
+
+(** TODO: Why is this failing? **)
+val safe_plugin1 : file_descr -> IIO unit pi (fun _ -> true) (fun _ _ _ -> true)
+let safe_plugin1 = safe_import plugin1
